LiveVerif/src/LiveVerifExamples/ErrorTests/if_while_scoping.v
@@ -1,0 +1,79 @@
+(* -*- eval: (load-file "../../LiveVerif/live_verif_setup.el"); -*- *)
+Require Import LiveVerif.LiveVerifLib.
+
+Ltac pose_err e ::= pose_err_silent e.
+
+Load LiveVerif.
+
+#[export] Instance spec_of_test_local_from_branches: fnspec := .**/
+
+uintptr_t test_local_from_branches(uintptr_t px, uintptr_t py) /**#
+  ghost_args := (R: mem -> Prop) x1 x2 y1 y2;
+  requires t m := <{ * uint 32 (x1 + x2) px
+                     * uint 32 (y1 + y2) py
+                     * R }> m;
+  ensures t' m' retv := t' = t /\
+            <{ * uint 32 (x1 + x2) px
+               * uint 32 (y1 + y2) py
+               * R }> m' #**/                                              /**.
+Derive test_local_from_branches SuchThat
+   (fun_correct! test_local_from_branches) As test_local_from_branches_ok.      .**/
+{                                                                          /**. .**/
+  uintptr_t g = 0;                                                         /**. .**/
+  if (load32(px) < load32(py)) {                                           /**. .**/
+    uintptr_t r = load32(px);                                              /**. .**/
+    g = r + 1;                                                             /**. .**/
+  } else {                                                                 /**. .**/
+    uintptr_t r = load32(py);                                              /**. .**/
+    g = r - 1;                                                             /**. .**/
+  } /**. end if.
+
+  lazymatch goal with
+  | |- @ready (wp_cmd ?fs ?c ?t ?m (map.of_list [|("g", g); ("px", px); ("py", py)|]) ?post)
+    => idtac (* note that the list of locals does not contain r, even though it was
+                added in both branches *)
+  end.
+
+  assert_fails (idtac; .**/ return r; /** ).
+  .**/ return g; /**.
+  .**/ } /**.
+Qed.
+
+#[export] Instance spec_of_test_local_from_loop_body: fnspec := .**/
+
+uintptr_t test_local_from_loop_body(uintptr_t px) /**#
+  ghost_args := (R: mem -> Prop) x1 x2;
+  requires t m := <{ * uint 32 (x1 + x2) px
+                     * R }> m;
+  ensures t' m' retv := t' = t /\
+            <{ * uint 32 (x1 + x2) px
+               * R }> m' #**/                                              /**.
+Derive test_local_from_loop_body SuchThat
+   (fun_correct! test_local_from_loop_body) As test_local_from_loop_body_ok.    .**/
+{                                                                          /**. .**/
+  uintptr_t g = 0;                                                         /**. .**/
+  uintptr_t i = 0;                                                         /**.
+
+  assert (0 <= \[i] <= 10) by steps.
+  loop invariant above i.
+  swap /[0] with (i ^* i) in #(g = ??).
+  delete #(i = ??).
+                                                                                .**/
+  while (i < 10) /* decreases (10 - \[i]) */ {                             /**. .**/
+    i = i + 1;                                                             /**. .**/
+    uintptr_t t = i * i;                                                   /**. .**/
+    g = t;                                                                 /**. .**/
+  } /**. end while.
+  (* TODO: turn lower+upper bound into equality whenever possible *)
+
+  lazymatch goal with
+  | |- @ready (wp_cmd ?fs ?c ?t ?m (map.of_list [|("g", g); ("i", i); ("px", px)|]) ?post)
+    => idtac (* note that the list of locals does not contain t, but that's not
+                surprising because if no loop iteration is run at all, it's not set *)
+  end.
+                                                                                .**/
+  return g;                                                                /**. .**/
+}                                                                          /**.
+Qed.
+
+End LiveVerif. Comments .**/ //.
