LiveVerif/src/LiveVerifExamples/Tests/if_merging.v
@@ -1,0 +1,31 @@
+(* -*- eval: (load-file "../../LiveVerif/live_verif_setup.el"); -*- *)
+Require Import LiveVerif.LiveVerifLib.
+
+Ltac pose_err e ::= pose_err_silent e.
+
+Load LiveVerif.
+
+#[export] Instance spec_of_test_if: fnspec :=                                .**/
+
+uintptr_t test_if(uintptr_t px, uintptr_t py) /**#
+  ghost_args := (R: mem -> Prop) x1 x2 y1 y2;
+  requires t m := <{ * uint 32 (x1 + x2) px
+                     * uint 32 (y1 + y2) py
+                     * R }> m;
+  ensures t' m' retv := t' = t /\
+            <{ * uint 32 (x1 + x2) px
+               * uint 32 (y1 + y2) py
+               * R }> m' #**/                                              /**.
+Derive test_if SuchThat (fun_correct! test_if) As test_if_ok.                   .**/
+{                                                                          /**. .**/
+  uintptr_t r = 0;                                                         /**. .**/
+  if (load32(px) < load32(py)) {                                           /**. .**/
+    r = load32(px);                                                        /**. .**/
+  } else {                                                                 /**. .**/
+    r = load32(py);                                                        /**. .**/
+  } /**. end if.                                                                .**/
+  return r;                                                                /**. .**/
+}                                                                          /**.
+Qed.
+
+End LiveVerif. Comments .**/ //.
